VecUtils.v
@@ -1,0 +1,92 @@
+Require Import Logic.Eqdep_dec.
+Require Import PeanoNat.
+Require Vectors.VectorDef.
+
+Definition vec := VectorDef.t.
+
+Section vec_all.
+  Variable A : Type.
+  Variable P : A -> Prop.
+
+  Fixpoint vec_all {n} (v : vec A n) :=
+    match v with
+    | VectorDef.nil _ => True
+    | VectorDef.cons _ a _ v' => P a /\ vec_all v'
+    end.
+
+  Definition vec_all_nil : vec_all (VectorDef.nil _) := I.
+
+  Lemma vec_all_singleton a
+    : P a -> vec_all (VectorDef.cons _ a _ (VectorDef.nil _)).
+  Proof.
+    unfold vec_all. auto.
+  Qed.
+
+  Lemma vec_all_cons a {n} (v : vec A n)
+    : P a -> vec_all v -> vec_all (VectorDef.cons _ a _ v).
+  Proof.
+    intros aH vH.
+    unfold vec_all; fold (@vec_all n).
+    exact (conj aH vH).
+  Qed.
+
+  Lemma not_vec_all_cons0 a {n} (v : vec A n)
+    : ~ P a -> ~ vec_all (VectorDef.cons _ a _ v).
+  Proof.
+    intro naH; unfold vec_all; fold (@vec_all n); tauto.
+  Qed.
+
+  Lemma not_vec_all_cons1 a {n} (v : vec A n)
+    : ~ vec_all v -> ~ vec_all (VectorDef.cons _ a _ v).
+  Proof.
+    unfold vec_all at 2; fold (@vec_all n); tauto.
+  Qed.
+End vec_all.
+
+Arguments vec_all {A} P {n}.
+Arguments vec_all_nil {A} P.
+Arguments vec_all_singleton {A P a} aH.
+Arguments vec_all_cons {A P a n v} aH vH.
+Arguments not_vec_all_cons0 {A P a n v} naH.
+Arguments not_vec_all_cons1 {A P} a {n v} nvH.
+
+Section dec_vec_all.
+  Variable A : Type.
+  Variable P : A -> Prop.
+  Hypothesis decP : forall x : A, {P x} + {~ (P x)}.
+
+  Fixpoint dec_vec_all {n} (v : vec A n) : {vec_all P v} + {~ (vec_all P v)} :=
+    match v with
+    | VectorDef.nil _ => left (vec_all_nil P)
+    | VectorDef.cons _ a _ v' =>
+      match decP a with
+      | left paH => match dec_vec_all v' with
+                    | left restH => left (vec_all_cons paH restH)
+                    | right nrestH => right (not_vec_all_cons1 a nrestH)
+                    end
+      | right nH => right (not_vec_all_cons0 nH)
+      end
+    end.
+End dec_vec_all.
+
+Arguments dec_vec_all {A P} decP {n} v.
+
+Section dec_vec.
+  Variable A : Type.
+  Hypothesis decA : forall x y : A, {x = y} + {x <> y}.
+
+  Definition dec_vec {n} (v v' : vec A n) : {v = v'} + {v <> v'}.
+    refine (VectorDef.rect2 (fun _ x y => {x = y} + {x <> y})
+                            (left (eq_refl))
+                            (fun n v v' veq a a' => _)
+                            v v').
+    - destruct (decA a a') as [ eqaH | neaH ].
+      + rewrite <- eqaH; clear eqaH a'.
+        destruct veq as [ eqvH | nevH ].
+        * rewrite <- eqvH. apply left. exact eq_refl.
+        * apply right. intro consH. inversion consH.
+          exact (nevH (inj_pair2_eq_dec nat Nat.eq_dec (vec A) n v v' H0)).
+      + apply right.
+        intro consH. inversion consH. contradiction.
+  Defined.
+End dec_vec.
